MIRification

Definitions.thy
@@ -20,6 +20,7 @@ type_synonym vname = string
 datatype ty = Tbool | Tint | Tref ty
 type_synonym tag = nat
 type_synonym address = nat
+datatype tag_kind = Unique
 
 text \<open>References consists of the address of the referent and the tag.
 A unique tag is assigned to each reference on creation.\<close>
@@ -28,34 +29,65 @@ datatype val = VBool bool | VInt int | Reference address tag
 
 subsection \<open>Expressions\<close>
 
-datatype 
-  exp = Const val
-  | Var vname
-  | Box exp
-  | Reborrow exp
-  | Deref exp
-  | Plus exp exp
-  | Less exp exp
-  | Not exp
-  | And exp exp
+datatype place = Var vname | Deref place
 
-text \<open>@{const_typ Box} allocates memory in the heap, initializing with the argument
+text \<open>Datatype @{typ place} represents an access path to data.
+It corresponds to \rust{Place} in \<^url>\<open>https://doc.rust-lang.org/nightly/nightly-rustc/rustc_middle/mir/struct.Place.html\<close>\<close>
+
+datatype operand = Place place | Constant val
+
+text \<open>Datatype @{typ operand} describes a value inside an rvalue.
+\<^term>\<open>Place\<close> denotes the current value at the place, while \<^term>\<open>Constant\<close> denotes a constant value.
+@{typ operand} corrensponds to \rust{Place} in \<^url>\<open>https://doc.rust-lang.org/nightly/nightly-rustc/rustc_middle/mir/enum.Operand.html\<close>,
+though we simplified the differentiation between a move and a copy
+(i.e. Unique doesn't track the ownership).\<close>
+
+datatype
+  rvalue = Use operand
+  | Box operand
+  | Ref place
+  | Reborrow place
+  | Plus operand operand
+  | Less operand operand
+  | Not operand
+  | And operand operand
+
+text \<open>Datatype @{typ rvalue} corresponds to an expression in a usual programming language
+(as in the previous version of Unique).
+We chose the term rvalue because of parity with Rust MIR
+(\<^url>\<open>https://doc.rust-lang.org/nightly/nightly-rustc/rustc_middle/mir/enum.Rvalue.html\<close>)
+
+Note that @{typ rvalue} is \<^emph>\<open>not\<close> recursive.
+Compound expressions need to be broken apart so that intermediate computation is stored to a variable.
+\<close>
+
+text \<open>
+The semantics of the constructs is as follows:
+\<^item> @{const_typ Box} allocates memory in the heap, initializing with the argument
 (\rust{Box::new} in Rust). @{const Box} returns a new unique reference.
-@{const_typ Reborrow} creates a new unique reference reborrowing from the argument
+Note that Box in MIR doesn't initialize the location but only allocates.
+The semantics will be adapted to MIR's one as we formalize uninitialized memory.
+\<^item> @{const_typ Ref} creates a unique reference pointing to the place.
+\<^item> @{const_typ Reborrow} creates a new unique reference reborrowing from the argument
 (\rust{&mut *p} in Rust, although most of the reborrows are automatically inserted by Rust).
-@{const_typ Deref} retrieves the content from the heap the reference pointing to (\rust{*p} in Rust).\<close>
+(TODO: I guess \rust{Use(Copy(mutable ref))} in MIR corresponds to Reborrow in Unique. )
+\<close>
 
 subsection \<open>Commands\<close>
 
-datatype 
+datatype
   com = Skip
-  | VarAssign vname exp ("_ ::= _" [1000, 61] 61)
-  | HeapAssign exp exp  ("*_ ::= _" [1000, 61] 61)
+  | Assign place rvalue ("_ ::= _" [1000, 61] 61)
   | Seq com com         ("_;;/ _" [60, 61] 60)
-  | If exp com com      ("(IF _/ THEN _/ ELSE _)" [0, 0, 61] 61)
-  | WHILE exp com       ("(WHILE _/ DO _)" [0, 61] 61)
+  | If rvalue com com      ("(IF _/ THEN _/ ELSE _)" [0, 0, 61] 61)
+  | WHILE rvalue com       ("(WHILE _/ DO _)" [0, 61] 61)
 
-type_synonym gamma = "vname \<Rightarrow> val option"
+type_synonym gamma = "vname \<Rightarrow> address * tag"
+
+text \<open>Unique implicitly performs boxing to variables. In other words,
+every variable behaves as a root reference to a memory cell.\<close>
+
+type_synonym tags = "tag_kind list"
 type_synonym borrow_list = "tag list"
 type_synonym heap = "(val * borrow_list) list"
 
@@ -78,15 +110,16 @@ next
   then show ?case by auto
 qed
 
-lemma [simp]: "t \<in> set ts \<Longrightarrow> kill t ts \<noteq> []" \<^marker>\<open>tag invisible\<close>
-proof (induction ts) \<^marker>\<open>tag invisible\<close>
+(*<*)
+lemma [simp]: "t \<in> set ts \<Longrightarrow> kill t ts \<noteq> []"
+proof (induction ts)
   case (Cons t' ts)
   then show ?case
     by (metis kill.simps(2) list.case_eq_if list.distinct(1) set_ConsD)
 qed auto
 
-lemma kill_lemma: "kill t ts = ts' \<Longrightarrow> ts' = [] \<or> last ts' = t" \<^marker>\<open>tag invisible\<close>
-proof (induction ts arbitrary: ts') \<^marker>\<open>tag invisible\<close>
+lemma kill_lemma: "kill t ts = ts' \<Longrightarrow> ts' = [] \<or> last ts' = t"
+proof (induction ts arbitrary: ts')
   case Nil
   then show ?case by simp
 next
@@ -95,15 +128,15 @@ next
     by (metis (no_types, lifting) kill.simps(2) last.simps list.case_eq_if list.collapse)
 qed
 
-lemma [simp]: "t \<in> set ts \<Longrightarrow> last (kill t ts) = t" \<^marker>\<open>tag invisible\<close>
-proof - \<^marker>\<open>tag invisible\<close>
+lemma [simp]: "t \<in> set ts \<Longrightarrow> last (kill t ts) = t"
+proof -
   assume "t \<in> set ts"
   hence "kill t ts \<noteq> []" by simp
   thus "last (kill t ts) = t" using kill_lemma by auto
 qed
 
-lemma kill_lemma': "\<lbrakk>kill t ts = ts'; ts' \<noteq> []\<rbrakk> \<Longrightarrow> \<exists>ts''. ts' = ts'' @ [t]" \<^marker>\<open>tag invisible\<close>
-proof (induction ts arbitrary: ts') \<^marker>\<open>tag invisible\<close>
+lemma kill_lemma': "\<lbrakk>kill t ts = ts'; ts' \<noteq> []\<rbrakk> \<Longrightarrow> \<exists>ts''. ts' = ts'' @ [t]"
+proof (induction ts arbitrary: ts')
   case Nil
   then show ?case by simp
 next
@@ -111,6 +144,7 @@ next
   then show ?case
     by (metis kill_lemma snoc_eq_iff_butlast)
 qed
+(*>*)
 
 lemma "t \<in> set ts \<Longrightarrow> \<exists>ts'. kill t ts = ts' @ [t]"
 proof -
@@ -119,22 +153,77 @@ proof -
   thus "\<exists>ts'. kill t ts = ts' @ [t]" using kill_lemma' by auto
 qed
 
-fun tags :: "heap \<Rightarrow> tag list" where
-  "tags H = fold (\<lambda>e ts. ts @ (snd e)) H []"
+fun kill_heap :: "(address * tag) \<Rightarrow> heap \<Rightarrow> heap" where
+  "kill_heap (a, t) H = (let (v, ts) = H ! a in H[a := (v, kill t ts)])"
+abbreviation kill_all :: "(address * tag) list \<Rightarrow> heap \<Rightarrow> heap" where
+  "kill_all refs H == foldr kill_heap refs H"
 
-fun fresh_tag :: "heap \<Rightarrow> tag" where
-  "fresh_tag H = fold max (tags H) 0 + 1"
-
-text \<open>Function @{const_typ fresh_tag} generates a new tag which doesn't exist in the tree.
-(FIXME: I figure that @{const fresh_tag} may reuse tags if they have been already killed.
-We need to record all the tags generated.)\<close>
-
-fun writable :: "address \<Rightarrow> tag \<Rightarrow> heap \<Rightarrow> bool" where
-  "writable p t H \<longleftrightarrow> p < length H \<and> t \<in> set (snd (H ! p))"
+fun writable :: "heap \<Rightarrow> (address * tag) \<Rightarrow> bool" where
+  "writable H (p, t) \<longleftrightarrow> p < length H \<and> t \<in> set (snd (H ! p))"
 definition "readable" where "readable = writable"
 
 text \<open>Functions @{const_typ writable} and @{const_typ readable} determine whether the given reference
 can be used to write to/read from it. The validity of references is determined by the existence in the current borrow tree.
 In Unique, we allow only unique references. Thus @{const readable} is equivalent to @{const writable}.\<close>
+
+definition allocated :: "heap \<Rightarrow> address \<Rightarrow> bool" where
+  "allocated H a \<longleftrightarrow> a < length H"
+
+(*<*)
+lemma kill_all_head: "kill_all (h # t) H = kill_heap h (kill_all t H)" by simp
+lemma kill_all_append[simp]: "kill_all (l1 @ l2) H = kill_all l1 (kill_all l2 H)" by simp
+
+lemma kill_preserve_length: "\<lbrakk>length H = l; H' = kill_heap (a, t) H\<rbrakk> \<Longrightarrow> length H' = l"
+  by (simp add: prod.case_eq_if)
+
+lemma kill_all_preserve_length: "\<lbrakk>length H = l; H' = kill_all refs H\<rbrakk> \<Longrightarrow> length H' = l"
+proof (induction refs arbitrary: l H H')
+  case Nil
+  then show ?case by simp
+next
+  case (Cons h t)
+  moreover have "H' = kill_heap h (kill_all t H)" using calculation(3) kill_all_head by blast
+  moreover have "length (kill_all t H) = l" using Cons.IH calculation(2) by blast
+  moreover have "length H' = l"
+    by (metis Cons.IH calculation(2) calculation(3) kill_all_head
+              kill_heap.elims kill_preserve_length)
+  ultimately show ?case by simp
+qed
+
+lemma kill_preserve_allocated: "\<lbrakk>allocated H a; H' = kill_heap (a, t) H\<rbrakk> \<Longrightarrow> allocated H' a"
+  using allocated_def kill_preserve_length by force
+
+lemma kill_all_preserve_allocated: "\<lbrakk>allocated H a; H' = kill_all refs H\<rbrakk> \<Longrightarrow> allocated H' a"
+  using allocated_def kill_all_preserve_length by force
+
+lemma kill_heap_access: "\<lbrakk>allocated H a; H ! a = (v, ts); H' = kill_heap (a', t) H\<rbrakk> \<Longrightarrow>
+  H' ! a = (if a = a' then (v, kill t ts) else (v, ts))"
+  by (smt allocated_def fst_conv kill_heap.simps nth_list_update_eq
+          nth_list_update_neq prod.case_eq_if snd_conv)
+
+lemma "\<lbrakk>allocated H a; H' = kill_all refs H\<rbrakk> \<Longrightarrow>
+  H' ! a = foldr (\<lambda>(a', t) (v, ts). if a = a' then (v, kill t ts) else (v, ts)) refs (H ! a)"
+proof (induction refs arbitrary: H')
+  case Nil
+  then show ?case by auto
+next
+  case (Cons ata refs H')
+  obtain aa ta where ata: "ata = (aa, ta)" by fastforce
+  let ?H = "kill_all refs H"
+  let ?f = "\<lambda>(a', t) (v, ts). if a = a' then (v, kill t ts) else (v, ts)"
+
+  have "?H ! a = foldr ?f refs (H ! a)" using Cons.IH Cons.prems by blast
+  moreover obtain v ts where vts: "?H ! a = (v, ts)" by fastforce
+  moreover have mid: "foldr ?f refs (H ! a) = (v, ts)" using calculation by auto
+  ultimately have rhs: "foldr ?f (ata # refs) (H ! a) = ?f ata (v, ts)" by (simp add: mid)
+
+  assume "H' = kill_all (ata # refs) H"
+  then have "H' = kill_heap (aa, ta) (kill_all refs H)" using ata by auto
+  then have lhs: "H' ! a = (if a = aa then (v, kill ta ts) else (v, ts))"
+    using Cons.prems(1) kill_all_preserve_allocated kill_heap_access vts by auto
+
+  from lhs rhs show "H' ! a = foldr ?f (ata # refs) (H ! a)" by (simp add: ata)
+qed
+(*>*)
 
 end
