Exp.thy
@@ -6,24 +6,89 @@ section \<open>Semantics of Expressions\<close>
 
 text \<open>This section presents the big-step semantics of expressions.\<close>
 
-inductive exp_sem :: 
-  "gamma * heap * exp \<Rightarrow> heap * val \<Rightarrow> bool" (infix "\<Down>" 65)
+inductive place_sem ::
+  "gamma \<Rightarrow> heap \<Rightarrow> place \<Rightarrow> (address * tag) list * val \<Rightarrow> bool"
+  ("(_; _ \<turnstile> _ \<Down>\<^sub>p _)")
 where
-  Const: "(\<Gamma>, H, Const v) \<Down> (H, v)" |
-  Var: "the (\<Gamma> x) = v \<Longrightarrow> (\<Gamma>, H, Var x) \<Down> (H, v)" |
-  Box: "\<lbrakk>(\<Gamma>, H, e) \<Down> (H', v); p = length H'; t = fresh_tag H'\<rbrakk> 
-        \<Longrightarrow> (\<Gamma>, H, Box e) \<Down> (H' @ [(v, [t])], Reference p t)" |
-  Reborrow: "\<lbrakk>(\<Gamma>, H, e) \<Down> (H', Reference p t); writable p t H'; (v, ts) = H' ! p; t' = fresh_tag H'\<rbrakk>
-             \<Longrightarrow> (\<Gamma>, H, Reborrow e) \<Down> (H'[p := (v, (kill t ts) @ [t'])], Reference p t')" |
-  Deref: "\<lbrakk>(\<Gamma>, H, e) \<Down> (H', Reference p t); readable p t H'; (v, ts) = H' ! p\<rbrakk>
-          \<Longrightarrow> (\<Gamma>, H, Deref e) \<Down> (H'[p := (v, kill t ts)], v)" |
-  Plus: "\<lbrakk>(\<Gamma>, H, e1) \<Down> (H', VInt i1); (\<Gamma>, H', e2) \<Down> (H'', VInt i2)\<rbrakk>
-         \<Longrightarrow> (\<Gamma>, H, Plus e1 e2) \<Down> (H'', VInt (i1 + i2))" |
-  Less: "\<lbrakk>(\<Gamma>, H, e1) \<Down> (H', VInt i1); (\<Gamma>, H', e2) \<Down> (H'', VInt i2)\<rbrakk>
-         \<Longrightarrow> (\<Gamma>, H, Less e1 e2) \<Down> (H'', VBool (i1 < i2))" |
-  Not: "(\<Gamma>, H, e) \<Down> (H', VBool b) \<Longrightarrow> (\<Gamma>, H, Not e) \<Down> (H', VBool (\<not>b))" |
-  And: "\<lbrakk>(\<Gamma>, H, e1) \<Down> (H', VBool b1); (\<Gamma>, H', e2) \<Down> (H'', VBool b2)\<rbrakk>
-         \<Longrightarrow> (\<Gamma>, H, And e1 e2) \<Down> (H'', VBool (b1 \<and> b2))"
+  Var: "\<Gamma> x = (a, t) \<Longrightarrow> \<Gamma>; H \<turnstile> Var x \<Down>\<^sub>p ([], Reference a t)" |
+  Deref: "\<lbrakk>\<Gamma>; H \<turnstile> p \<Down>\<^sub>p (refs, Reference a t); allocated H a\<rbrakk> \<Longrightarrow>
+          \<Gamma>; H \<turnstile> Deref p \<Down>\<^sub>p ((a, t) # refs, fst (H ! a))"
+
+text \<open>The relation @{const place_sem} describes the semantics of places.
+\<^term>\<open>\<Gamma>; H \<turnstile> p \<Down>\<^sub>p (refs, v)\<close> means that a place expression \<^term>\<open>p\<close> evaluates to
+a value \<^term>\<open>v\<close> under the environment \<^term>\<open>\<Gamma>\<close> and \<^term>\<open>H\<close>, where \<^term>\<open>refs\<close> are
+the references used to retrieve the value (thus they need to be validated).\<close>
+
+(*<*)
+lemmas place_sem_cases = place_sem.cases[split_format(complete)]
+lemmas place_sem_induct = place_sem.induct[split_format(complete)]
+declare place_sem.intros[simp, intro]
+inductive_cases place_sem_inv[elim!]:
+  "\<Gamma>; H \<turnstile> Var x \<Down>\<^sub>p (refs, v)"
+  "\<Gamma>; H \<turnstile> Deref p \<Down>\<^sub>p (refs, v)"
+(*>*)
+
+inductive operand_sem ::
+  "gamma \<Rightarrow> heap \<Rightarrow> operand \<Rightarrow> (address * tag) list * val \<Rightarrow> bool"
+  ("(_; _ \<turnstile> _ \<Down>\<^sub>o\<^sub>p _)")
+where
+  Place: "\<Gamma>; H \<turnstile> p \<Down>\<^sub>p v \<Longrightarrow> \<Gamma>; H \<turnstile> Place p \<Down>\<^sub>o\<^sub>p v" |
+  Constant: "\<Gamma>; H \<turnstile> Constant v \<Down>\<^sub>o\<^sub>p ([], v)"
+
+(*<*)
+lemmas operand_sem_cases = operand_sem.cases[split_format(complete)]
+lemmas operand_sem_induct = operand_sem.induct[split_format(complete)]
+declare operand_sem.simps[simp, intro]
+inductive_cases operand_sem_inv[elim!]:
+  "\<Gamma>; H \<turnstile> Place p \<Down>\<^sub>o\<^sub>p v"
+  "\<Gamma>; H \<turnstile> Constant v \<Down>\<^sub>o\<^sub>p v'"
+(*>*)
+
+inductive rvalue_sem ::
+  "gamma * tags * heap * rvalue \<Rightarrow> tags * heap * val \<Rightarrow> bool" (infix "\<Down>" 65)
+where
+  Use: "\<lbrakk>\<Gamma>; H \<turnstile> op \<Down>\<^sub>o\<^sub>p (refs, v); list_all (readable H) refs\<rbrakk>
+        \<Longrightarrow> (\<Gamma>, T, H, Use op) \<Down> (T, kill_all refs H, v)" |
+  Box: "\<lbrakk>\<Gamma>; H \<turnstile> op \<Down>\<^sub>o\<^sub>p (refs, v); p = length H; t = length T\<rbrakk>
+        \<Longrightarrow> (\<Gamma>, T, H, Box op) \<Down> (T @ [Unique], H @ [(v, [t])], Reference p t)" |
+  Ref: "\<lbrakk>\<Gamma>; H \<turnstile> p \<Down>\<^sub>p (refs, Reference a t); list_all (readable H) refs\<rbrakk>
+        \<Longrightarrow> (\<Gamma>, T, H, Ref p) \<Down> (T, kill_all refs H, Reference a t)" |
+  Reborrow: "\<lbrakk>\<Gamma>; H \<turnstile> p \<Down>\<^sub>p (refs, Reference a t); list_all (writable H) refs;
+              writable H (a, t); t' = length T;
+              H' = kill_all ((a, t) # refs) H; H' ! a = (v, ts)\<rbrakk>
+             \<Longrightarrow> (\<Gamma>, T, H, Reborrow p) \<Down> (T @ [Unique], H'[a := (v, ts @ [t'])] , Reference a t')" |
+  Plus: "\<lbrakk>\<Gamma>; H \<turnstile> lhs \<Down>\<^sub>o\<^sub>p (rl, VInt lhs'); \<Gamma>; H \<turnstile> rhs \<Down>\<^sub>o\<^sub>p (rr, VInt rhs');
+          list_all (readable H) rl; list_all (readable H) rr\<rbrakk>
+         \<Longrightarrow> (\<Gamma>, T, H, Plus lhs rhs) \<Down> (T, kill_all (rr @ rl) H, VInt (lhs' + rhs'))" |
+  Less: "\<lbrakk>\<Gamma>; H \<turnstile> lhs \<Down>\<^sub>o\<^sub>p (rl, VInt lhs'); \<Gamma>; H \<turnstile> rhs \<Down>\<^sub>o\<^sub>p (rr, VInt rhs');
+          list_all (readable H) rl; list_all (readable H) rr\<rbrakk>
+         \<Longrightarrow> (\<Gamma>, T, H, Less lhs rhs) \<Down> (T, kill_all (rr @ rl) H, VBool (lhs' < rhs'))" |
+  Not: "\<lbrakk>\<Gamma>; H \<turnstile> op \<Down>\<^sub>o\<^sub>p (refs, VBool v); list_all (readable H) refs\<rbrakk>
+         \<Longrightarrow> (\<Gamma>, T, H, Not op) \<Down> (T, kill_all refs H, VBool (\<not>v))" |
+  And: "\<lbrakk>\<Gamma>; H \<turnstile> lhs \<Down>\<^sub>o\<^sub>p (rl, VBool lhs'); \<Gamma>; H \<turnstile> rhs \<Down>\<^sub>o\<^sub>p (rr, VBool rhs');
+          list_all (readable H) rl; list_all (readable H) rr\<rbrakk>
+         \<Longrightarrow> (\<Gamma>, T, H, And lhs rhs) \<Down> (T, kill_all (rr @ rl) H, VBool (lhs' \<and> rhs'))"
+
+(*<*)
+lemmas rvalue_sem_cases = rvalue_sem.cases[split_format(complete)]
+lemmas rvalue_sem_induct = rvalue_sem.induct[split_format(complete)]
+declare rvalue_sem.intros[simp, intro]
+inductive_cases rvalue_sem_inv[elim!]:
+  "(\<Gamma>, T, H, Use op) \<Down> (T', H', v)"
+  "(\<Gamma>, T, H, Box op) \<Down> (T', H', v)"
+  "(\<Gamma>, T, H, Ref p) \<Down> (T', H', v)"
+  "(\<Gamma>, T, H, Reborrow p) \<Down> (T', H', v)"
+  "(\<Gamma>, T, H, Plus lhs rhs) \<Down> (T', H', v)"
+  "(\<Gamma>, T, H, Less lhs rhs) \<Down> (T', H', v)"
+  "(\<Gamma>, T, H, Not op) \<Down> (T', H', v)"
+  "(\<Gamma>, T, H, And lhs rhs) \<Down> (T', H', v)"
+(*>*)
+
+text \<open>
+Some TODO notes on the semantics of expressions:
+\<^item> I don't get the semantics of @{const Ref} in MIR and how it should behave under the auto-boxing of variables.
+\<^item> I'm not sure readable/writable checking is correct.
+\<close>
 
 text \<open>
 We present the intuition behind the selected rules.
@@ -35,17 +100,17 @@ returning a reference pointing to the slot with a fresh tag.
 @{thm[mode=Rule] Box} \sc{Box}
 \end{framed}
 
-Next, {\sc{Deref}} rule allows us to access the content the given reference is pointing to.
-The validity of the reference is checked by @{const_typ readable}.
-Moreover, {\sc{Deref}} invalidates all descendant references to establish the uniqueness
-($kill\ t\ ts$).
+Next, {\sc{Use}} and {\sc{Ref}} rules allow us to read the content through a place (or give a constant).
+The validity of the access is checked by @{const_typ readable}.
+Moreover, they invalidate all descendant references to establish the uniqueness.
 
 \begin{framed}
 \centering
-@{thm[mode=Rule] Deref} \sc{Deref}
+@{thm[mode=Rule] Use} \sc{Use}\\
+@{thm[mode=Rule] Ref} \sc{Ref}
 \end{framed}
 
-Last but not least, {\sc{Reborrow}} rule creates a new reference with a fresh tag reborrowing the given reference.
+Last but not least, {\sc{Reborrow}} rule creates a new reference pointing to the same object but with a fresh tag.
 The newly created reference is writable. Thus the original reference must be valid for writes.
 Reborrow is considered as the use of the original reference and hence it invalidates former children
 of the reference. As a result, the reborrow tree will have the original reference and the reborrowing
@@ -58,76 +123,172 @@ reference as the last two element.
 \end{framed}
 \<close>
 
-(* proof automation *)
-(*<*)
-lemmas exp_sem_cases = exp_sem.cases[split_format(complete)] \<^marker>\<open>tag invisible\<close>
-lemmas exp_sem_induct = exp_sem.induct[split_format(complete)] \<^marker>\<open>tag invisible\<close>
-declare exp_sem.intros[simp, intro] \<^marker>\<open>tag invisible\<close>
-
-inductive_cases ConstE[elim!]: "(\<Gamma>, H, Const v) \<Down> v'" \<^marker>\<open>tag invisible\<close>
-inductive_cases VarE[elim!]: "(\<Gamma>, H, Var x) \<Down> v" \<^marker>\<open>tag invisible\<close>
-inductive_cases BoxE[elim!]: "(\<Gamma>, H, Box e) \<Down> v" \<^marker>\<open>tag invisible\<close>
-inductive_cases ReborrowE[elim!]: "(\<Gamma>, H, Reborrow e) \<Down> v" \<^marker>\<open>tag invisible\<close>
-inductive_cases DerefE[elim!]: "(\<Gamma>, H, Deref e) \<Down> v" \<^marker>\<open>tag invisible\<close>
-inductive_cases AlithE[elim!]: \<^marker>\<open>tag invisible\<close>
-  "(\<Gamma>, H, Plus e1 e2) \<Down> v"
-  "(\<Gamma>, H, Less e1 e2) \<Down> v"
-  "(\<Gamma>, H, Not e) \<Down> v"
-  "(\<Gamma>, H, And e1 e2) \<Down> v"
-
-(*>*)
-
-lemma reborrow_det_lemma: \<^marker>\<open>tag invisible\<close>
-  assumes
-    reborrow: "(\<Gamma>, H, Reborrow e) \<Down> E''" and
-    memory: "(v, ts) = H' ! p" and
-    readable: "readable p t H'" and
-    fresh_tag: "t' = fresh_tag H'" and
-    IH: "\<And>E'. (\<Gamma>, H, e) \<Down> E' \<Longrightarrow> E' = (H', Reference p t)"
-  shows "E'' = (H'[p := (v, kill t ts @ [t'])], Reference p t')"
-proof (rule ReborrowE[where \<Gamma> = \<Gamma> and H = H and v = E'' and e = e]) \<^marker>\<open>tag invisible\<close>
-  show "(\<Gamma>, H, Reborrow e) \<Down> E''" using reborrow by auto
-next
-  fix H'a pa ta va tsa
-  let ?fix_type = "fresh_tag H'a" (* without this line, the following let fails *)
-  let ?t'a = "Suc (fold max (fold (\<lambda>e ts. ts @ snd e) H'a []) 0)"
-  assume
-    e'': "E'' = (H'a[pa := (va, kill ta tsa @ [?t'a])], Reference pa ?t'a)" and
-    loc: "(\<Gamma>, H, e) \<Down>  (H'a, Reference pa ta)" and
-    memorya: "(va, tsa) = H'a ! pa" and
-    allocateda: "pa < length H'a" and
-    valida: "ta \<in> set (snd (H'a ! pa))"
-  moreover have "H'a = H'" "pa = p" "ta = t" using loc IH by auto
-  moreover have "(va, tsa) = (v, ts)" using calculation memory memorya by auto
-  moreover have "va = v" using calculation(9) by auto
-  moreover have "tsa = ts" using calculation(9) by auto
-  moreover have "?t'a = t'" using calculation(6) fresh_tag by auto
-  ultimately show "E'' = (H'[p := (v, kill t ts @ [t'])], Reference p t')" by auto
-qed
-
 text \<open>We can prove that the semantics of expressions is deterministic.\<close>
 
-lemma exp_sem_deterministic: "E \<Down> E' \<Longrightarrow> E \<Down> E'' \<Longrightarrow> E'' = E'"
-proof (induction E E' arbitrary: E'' rule: exp_sem.induct)
-  case (Reborrow \<Gamma> H e H' p t v ts t')
-  show ?case
-    using Reborrow.IH Reborrow.hyps(2) Reborrow.hyps(3) Reborrow.hyps(4)
-          Reborrow.prems readable_def reborrow_det_lemma by auto
+lemma place_sem_det: "\<Gamma>; H \<turnstile> p \<Down>\<^sub>p (refs, v) \<Longrightarrow> \<Gamma>; H \<turnstile> p \<Down>\<^sub>p (refs', v') \<Longrightarrow> (refs', v') = (refs, v)"
+proof (induction arbitrary: refs' v' rule: place_sem.induct)
+  case (Var \<Gamma> x a t H)
+  then show ?case by auto
 next
-  case (Deref \<Gamma> H e H' p t v ts)
-  then show ?case
-    by (smt DerefE Pair_inject val.inject(3))
-qed auto
+  case (Deref \<Gamma> H p refs a t)
+  then show ?case by blast
+qed
+lemmas place_sem_det' = place_sem_det[split_format(complete)]
 
-text \<open>The following lemmas are a sanity check of the semantics.
+lemma operand_sem_det: "\<Gamma>; H \<turnstile> op \<Down>\<^sub>o\<^sub>p (refs, v) \<Longrightarrow> \<Gamma>; H \<turnstile> op \<Down>\<^sub>o\<^sub>p (refs', v') \<Longrightarrow> (refs', v') = (refs, v)"
+proof (induction arbitrary: refs' v' rule: operand_sem.induct)
+  case (Place \<Gamma> H p v)
+  then show ?case
+    by (metis operand_sem_inv(1) place_sem_det' surj_pair)
+next
+  case (Constant \<Gamma> H v)
+  then show ?case by blast
+qed
+lemmas operand_sem_det' = operand_sem_det[split_format(complete)]
+
+lemma rvalue_sem_det: "(\<Gamma>, T, H, rv) \<Down> (T', H', v') \<Longrightarrow> (\<Gamma>, T, H, rv) \<Down> (T'', H'', v'')
+  \<Longrightarrow> (T'', H'', v'') = (T', H', v')"
+proof (induction rule: rvalue_sem_induct)
+  case (Use \<Gamma> H op refs v T)
+  show "(T'', H'', v'') = (T, kill_all refs H, v)"
+  proof (rule rvalue_sem_inv(1))
+    fix refs'
+    assume op: "(\<exists>p. op = Place p \<and> (\<Gamma>; H \<turnstile> p \<Down>\<^sub>p (refs', v''))) \<or> op = Constant v'' \<and> refs' = []"
+    then have "\<Gamma>; H \<turnstile> op \<Down>\<^sub>o\<^sub>p (refs', v'')" by simp
+    then have "refs' = refs" and "v'' = v" using Use.hyps(1) operand_sem_det' by auto
+    then show "(T'', H'', v'') = (T, kill_all refs H, v)"
+      using Use.prems op place_sem_det' by blast
+  next
+    show "(\<Gamma>, T, H, Use op) \<Down> (T'', H'', v'')" using Use.prems by auto
+  qed
+next
+  case (Box \<Gamma> H op refs v p t T)
+  then show ?case using place_sem_det' by auto
+next
+  case (Ref \<Gamma> H p refs a t T)
+  then show ?case using place_sem_det' by fastforce
+next
+  case (Reborrow \<Gamma> H p refs a t t' T H' v ts)
+  show "(T'', H'', v'') = (T @ [Unique], H'[a := (v, ts @ [t'])], Reference a t')"
+  proof (rule rvalue_sem_inv(4))
+    show "(\<Gamma>, T, H, Reborrow p) \<Down> (T'', H'', v'')" using Reborrow.prems by simp
+  next
+    fix refsa aa ta va tsa
+    let ?kill = "(case kill_all refsa H ! aa of (va, tsa) \<Rightarrow> (kill_all refsa H)[aa := (va, kill ta tsa)])"
+    assume "\<Gamma>; H \<turnstile> p \<Down>\<^sub>p (refsa, Reference aa ta)"
+    then have "refsa = refs \<and> aa = a \<and> ta = t" using Reborrow.hyps place_sem_det' by blast
+    then have "refsa = refs" and "aa = a" and "ta = t" by auto
+    moreover assume "?kill ! aa = (va, tsa)"
+    then have "va = v" and "tsa = ts" using Reborrow.hyps calculation by auto
+    moreover assume "H'' = ?kill[aa := (va, tsa @ [length T])]"
+    then have "H'' = H'[a := (v, ts @ [t'])]" by (simp add: Reborrow.hyps calculation)
+    moreover assume "v'' = Reference aa (length T)"
+    then have "v'' = Reference a t'" using Reborrow.hyps calculation by simp
+    ultimately show ?thesis using Reborrow.prems by auto
+  qed
+next
+  case (Plus \<Gamma> H lhs rl lhs' rhs rr rhs' T)
+  show "(T'', H'', v'') = (T, kill_all (rr @ rl) H, VInt (lhs' + rhs'))"
+  proof (rule rvalue_sem_inv(5))
+    show "(\<Gamma>, T, H, Plus lhs rhs) \<Down> (T'', H'', v'')" using Plus.prems by simp
+  next
+    fix rla lhs'a rra rhs'a
+    assume opl: "(\<exists>p. lhs = Place p \<and> (\<Gamma>; H \<turnstile> p \<Down>\<^sub>p (rla, VInt lhs'a))) \<or>
+            lhs = Constant (VInt lhs'a) \<and> rla = []" and
+           opr: "(\<exists>p. rhs = Place p \<and> (\<Gamma>; H \<turnstile> p \<Down>\<^sub>p (rra, VInt rhs'a))) \<or>
+            rhs = Constant (VInt rhs'a) \<and> rra = []"
+    then have "\<Gamma>; H \<turnstile> lhs \<Down>\<^sub>o\<^sub>p (rla, VInt lhs'a)" and "\<Gamma>; H \<turnstile> rhs \<Down>\<^sub>o\<^sub>p (rra, VInt rhs'a)" by auto
+    then have "rla = rl \<and> lhs'a = lhs' \<and> rra = rr \<and> rhs'a = rhs'"
+      using Plus.hyps operand_sem_det' by blast
+    then have "rla = rl" and "lhs'a = lhs'" and "rra = rr" and "rhs'a = rhs'" by auto
+    moreover assume "H'' = kill_all rra (kill_all rla H)" and "v'' = VInt (lhs'a + rhs'a)"
+    then have "H'' = kill_all (rr @ rl) H" and "v'' = VInt (lhs' + rhs')"
+      using calculation foldr_append by auto
+    ultimately show ?thesis using Plus.prems by auto
+  qed
+next
+  case (Less \<Gamma> H lhs rl lhs' rhs rr rhs' T)
+  show "(T'', H'', v'') = (T, kill_all (rr @ rl) H, VBool (lhs' < rhs'))"
+  proof (rule rvalue_sem_inv(6))
+    show "(\<Gamma>, T, H, Less lhs rhs) \<Down> (T'', H'', v'')" using Less.prems by simp
+  next
+    fix rla lhs'a rra rhs'a
+    assume opl: "(\<exists>p. lhs = Place p \<and> (\<Gamma>; H \<turnstile> p \<Down>\<^sub>p (rla, VInt lhs'a))) \<or>
+            lhs = Constant (VInt lhs'a) \<and> rla = []" and
+           opr: "(\<exists>p. rhs = Place p \<and> (\<Gamma>; H \<turnstile> p \<Down>\<^sub>p (rra, VInt rhs'a))) \<or>
+            rhs = Constant (VInt rhs'a) \<and> rra = []"
+    then have "\<Gamma>; H \<turnstile> lhs \<Down>\<^sub>o\<^sub>p (rla, VInt lhs'a)" and "\<Gamma>; H \<turnstile> rhs \<Down>\<^sub>o\<^sub>p (rra, VInt rhs'a)" by auto
+    then have "rla = rl \<and> lhs'a = lhs' \<and> rra = rr \<and> rhs'a = rhs'"
+      using Less.hyps operand_sem_det' by blast
+    then have "rla = rl" and "lhs'a = lhs'" and "rra = rr" and "rhs'a = rhs'" by auto
+    moreover assume "H'' = kill_all rra (kill_all rla H)" and "v'' = VBool (lhs'a < rhs'a)"
+    then have "H'' = kill_all (rr @ rl) H" and "v'' = VBool (lhs' < rhs')"
+      using calculation foldr_append by auto
+    ultimately show ?thesis using Less.prems by auto
+  qed
+next
+  case (Not \<Gamma> H op refs v T)
+  show "(T'', H'', v'') = (T, kill_all refs H, VBool (\<not>v))"
+  proof (rule rvalue_sem_inv(7))
+    fix refsa va
+    assume "(\<exists>p. op = Place p \<and> (\<Gamma>; H \<turnstile> p \<Down>\<^sub>p (refsa, VBool va))) \<or> op = Constant (VBool va) \<and> refsa = []"
+    then show "(T'', H'', v'') = (T, kill_all refs H, VBool (\<not>v))"
+      using Not.prems Not.hyps operand_sem_det' place_sem_det' by blast
+  next
+    show "(\<Gamma>, T, H, Not op) \<Down> (T'', H'', v'')" using Not.prems by simp
+  qed
+next
+  case (And \<Gamma> H lhs rl lhs' rhs rr rhs' T)
+  show "(T'', H'', v'') = (T, kill_all (rr @ rl) H, VBool (lhs' \<and> rhs'))"
+  proof (rule rvalue_sem_inv(8))
+    show "(\<Gamma>, T, H, And lhs rhs) \<Down> (T'', H'', v'')" using And.prems by simp
+  next
+    fix rla lhs'a rra rhs'a
+    assume opl: "(\<exists>p. lhs = Place p \<and> (\<Gamma>; H \<turnstile> p \<Down>\<^sub>p (rla, VBool lhs'a))) \<or>
+            lhs = Constant (VBool lhs'a) \<and> rla = []" and
+           opr: "(\<exists>p. rhs = Place p \<and> (\<Gamma>; H \<turnstile> p \<Down>\<^sub>p (rra, VBool rhs'a))) \<or>
+            rhs = Constant (VBool rhs'a) \<and> rra = []"
+    then have "\<Gamma>; H \<turnstile> lhs \<Down>\<^sub>o\<^sub>p (rla, VBool lhs'a)" and "\<Gamma>; H \<turnstile> rhs \<Down>\<^sub>o\<^sub>p (rra, VBool rhs'a)" by auto
+    then have "rla = rl \<and> lhs'a = lhs' \<and> rra = rr \<and> rhs'a = rhs'"
+      using And.hyps operand_sem_det' by blast
+    then have "rla = rl" and "lhs'a = lhs'" and "rra = rr" and "rhs'a = rhs'" by auto
+    moreover assume "H'' = kill_all rra (kill_all rla H)" and "v'' = VBool (lhs'a \<and> rhs'a)"
+    then have "H'' = kill_all (rr @ rl) H" and "v'' = VBool (lhs' \<and> rhs')"
+      using calculation foldr_append by auto
+    ultimately show ?thesis using And.prems by auto
+  qed
+qed
+
+text \<open>The following lemmas are sanity checks of the semantics.
 We must be able to write through the references retrieved by {\sc{Box}} and {\sc{Reborrow}}\<close>
 
-lemma box__writable: "(\<Gamma>, H, Box e) \<Down> (H', Reference p t) \<Longrightarrow> writable p t H'"
+lemma box__writable: "(\<Gamma>, T, H, Box e) \<Down> (T', H', Reference a t) \<Longrightarrow> writable H' (a, t)"
   by auto
 
-lemma reborrow__writable: "(\<Gamma>, H, Reborrow e) \<Down> (H', Reference p t) \<Longrightarrow> writable p t H'"
-  by auto
+lemma reborrow__writable: "(\<Gamma>, T, H, Reborrow p) \<Down> (T', H', Reference a t) \<Longrightarrow> writable H' (a, t)"
+proof (rule rvalue_sem_inv(4))
+  assume "(\<Gamma>, T, H, Reborrow p) \<Down> (T', H', Reference a t)"
+  then show "(\<Gamma>, T, H, Reborrow p) \<Down> (T', H', Reference a t)" by auto
+next
+  fix refsa aa ta va tsa
+  let ?kill = "(case kill_all refsa H ! aa of (va, tsa) \<Rightarrow> (kill_all refsa H)[aa := (va, kill ta tsa)])"
+  assume "H' = ?kill[aa := (va, tsa @ [length T])]"
+    and "aa < length H"
+    and "?kill ! aa = (va, tsa)"
+  then have "H' ! aa = (va, tsa @ [length T])"
+    by (metis (no_types, lifting) kill_all_preserve_length length_list_update
+      nth_list_update_eq prod.case_eq_if)
+  moreover assume "Reference a t = Reference aa (length T)"
+  then have "aa = a" and "t = length T" by auto
+  ultimately have alen: "a < length H" and elem: "H' ! a = (va, tsa @ [t])"
+    using \<open>aa < length H\<close> by auto
 
-code_pred [show_modes] exp_sem .
+  assume "H' = ?kill[aa := (va, tsa @ [length T])]"
+  then have alen': "a < length H'"
+    using alen kill_all_preserve_length kill_preserve_length by force
+
+  have "t \<in> set (snd (H' ! a))" by (simp add: elem)
+  with alen' show ?thesis by auto
+qed
 
 end
