Unique.thy
@@ -5,67 +5,59 @@ begin
 section \<open>Semantics of Commands\<close>
 
 text \<open>This section describes the small-step semantics of commands.
-The configuration of an execution consists of
-\begin{itemize}
-  \item the variable environment $\Gamma$ (of type @{type gamma});
-  \item the heap $H$ (of type @{type heap}) which holds the actual data and the reborrow trees
+The configuration of an execution consists of:
+\<^item> the variable environment $\Gamma$ (of type @{type gamma});
+\<^item> the heap $H$ (of type @{type heap}) which holds the actual data and the reborrow trees
   for each address; and
-  \item the command to be executed $c$ (of type @{type com}).
-\end{itemize}\<close>
+\<^item> the command to be executed $c$ (of type @{type com}).
+\<close>
 
-type_synonym config = "gamma * heap * com"
-inductive com_sem :: "config \<Rightarrow> config \<Rightarrow> bool" (infix "\<rightarrow>" 65)
+type_synonym config = "tags * heap * com"
+inductive com_sem :: "gamma \<Rightarrow> config \<Rightarrow> config \<Rightarrow> bool" ("(_ \<turnstile> _ \<rightarrow> _)")
 where
-  VAssign: "(\<Gamma>, H, e) \<Down> (H', v)
-            \<Longrightarrow> (\<Gamma>, H, x ::= e) \<rightarrow> (\<Gamma>(x \<mapsto> v), H', Skip)" |
-  HAssign: "\<lbrakk>(\<Gamma>, H, e\<^sub>l) \<Down> (H', Reference p t);
-             (\<Gamma>, H', e\<^sub>v) \<Down> (H'', v);
-             writable p t H''\<rbrakk>
-            \<Longrightarrow> (\<Gamma>, H, *e\<^sub>l ::= e\<^sub>v) \<rightarrow> (\<Gamma>, H''[p := (v, kill t (snd (H'' ! p)))], Skip)" |
-  SeqL: "(\<Gamma>, H, Skip;; c) \<rightarrow> (\<Gamma>, H, c)" |
-  SeqR: "(\<Gamma>, H, c1) \<rightarrow> (\<Gamma>', H', c') \<Longrightarrow> (\<Gamma>, H, c1;; c2) \<rightarrow> (\<Gamma>', H', c';; c2)" |
-  IfTrue: "(\<Gamma>, H, b) \<Down> (H', VBool True)
-           \<Longrightarrow> (\<Gamma>, H, IF b THEN c1 ELSE c2) \<rightarrow> (\<Gamma>, H', c1)" |
-  IfFlase: "(\<Gamma>, H, b) \<Down> (H', VBool False)
-           \<Longrightarrow> (\<Gamma>, H, IF b THEN c1 ELSE c2) \<rightarrow> (\<Gamma>, H', c2)" |
-  While: "(\<Gamma>, H, WHILE b DO c) \<rightarrow> (\<Gamma>, H, IF b THEN (c;; WHILE b DO c) ELSE Skip)"
+  Assign: "\<lbrakk>\<Gamma>; H \<turnstile> p \<Down>\<^sub>p (refs, Reference a t); list_all (writable H) refs; writable H (a, t);
+            H' = kill_all refs H; (\<Gamma>, T, H', rv) \<Down> (T', H'', v); H'' ! a = (_, ts)\<rbrakk>
+           \<Longrightarrow> \<Gamma> \<turnstile> (T, H, p ::= rv) \<rightarrow> (T', H''[a := (v, kill t ts)], Skip)" |
+  SeqL: "\<Gamma> \<turnstile> (T, H, Skip;; c) \<rightarrow> (T, H, c)" |
+  SeqR: "\<Gamma> \<turnstile> (T, H, c1) \<rightarrow> (T', H', c') \<Longrightarrow> \<Gamma> \<turnstile> (T, H, c1;; c2) \<rightarrow> (T', H', c';; c2)" |
+  IfTrue: "(\<Gamma>, T, H, b) \<Down> (T', H', VBool True)
+           \<Longrightarrow> \<Gamma> \<turnstile> (T, H, IF b THEN c1 ELSE c2) \<rightarrow> (T', H', c1)" |
+  IfFalse: "(\<Gamma>, T, H, b) \<Down> (T', H', VBool False)
+           \<Longrightarrow> \<Gamma> \<turnstile> (T, H, IF b THEN c1 ELSE c2) \<rightarrow> (T', H', c2)" |
+  While: "\<Gamma> \<turnstile> (T, H, WHILE b DO c) \<rightarrow> (T, H, IF b THEN (c;; WHILE b DO c) ELSE Skip)"
 
-code_pred [show_modes] com_sem .
-
-lemmas com_sem_cases = com_sem.cases[split_format(complete)] \<^marker>\<open>tag invisible\<close>
-lemmas com_sem_induct = com_sem.induct[split_format(complete)] \<^marker>\<open>tag invisible\<close>
-
-declare com_sem.intros[simp, intro] \<^marker>\<open>tag invisible\<close>
+(*<*)
+lemmas com_sem_cases = com_sem.cases[split_format(complete)]
+lemmas com_sem_induct = com_sem.induct[split_format(complete)]
+declare com_sem.intros[simp, intro]
 
 (* We declare safe elimination rules (automatically applied I guess?) *)
-inductive_cases ComE[elim!]: \<^marker>\<open>tag invisible\<close>
-  "(\<Gamma>, H, x ::= e) \<rightarrow> cfg"
-  "(\<Gamma>, H, *e\<^sub>l ::= e\<^sub>v) \<rightarrow> cfg"
-  "(\<Gamma>, H, Skip;; c) \<rightarrow> cfg"
-  "(\<Gamma>, H, c1;; c2) \<rightarrow> cfg"
-  "(\<Gamma>, H, IF b THEN c1 ELSE c2) \<rightarrow> cfg"
+inductive_cases ComE[elim!]:
+  "\<Gamma> \<turnstile> (T, H, x ::= e) \<rightarrow> cfg"
+  "\<Gamma> \<turnstile> (T, H, Skip;; c) \<rightarrow> cfg"
+  "\<Gamma> \<turnstile> (T, H, c1;; c2) \<rightarrow> cfg"
+  "\<Gamma> \<turnstile> (T, H, IF b THEN c1 ELSE c2) \<rightarrow> cfg"
 
 (* WHILE might not terminate, so we declare it as an unsafe elimination rule *)
-inductive_cases WhileE[elim]: "(\<Gamma>, H, WHILE b DO c) \<rightarrow> cfg" \<^marker>\<open>tag invisible\<close>
+inductive_cases WhileE[elim]: "\<Gamma> \<turnstile> (T, H, WHILE b DO c) \<rightarrow> cfg"
+(*>*)
 
-abbreviation com_sem_steps :: "config \<Rightarrow> config \<Rightarrow> bool" (infix "\<rightarrow>\<^sup>*" 65) where
-  "cfg \<rightarrow>\<^sup>* cfg' == star com_sem cfg cfg'"
+abbreviation com_sem_steps :: "gamma \<Rightarrow> config \<Rightarrow> config \<Rightarrow> bool" ("(_ \<turnstile> _ \<rightarrow>\<^sup>* _)") where
+  "\<Gamma> \<turnstile> cfg \<rightarrow>\<^sup>* cfg' == star (com_sem \<Gamma>) cfg cfg'"
 
 text \<open>
 Figure \ref{fig:com} shows the assignment rules. Other commands are standard.
 
-The {\sc{VAssign}} rule assigns a value to the variable while
-the {\sc{HAssign}} rule to the location the reference on the left hand side is referring to.
+The {\sc{Assign}} rule assigns a value to the the location.
 To assign through a reference, the reference must be valid for writes.
 Moreover, the write is considered as a use of the reference; it will invalidate the child references.
 
 \begin{figure}[h]
 \centering
 \begin{framed}
-@{thm[mode=Rule] VAssign} \sc{VAssign} \\
-@{thm[mode=Rule] HAssign} \sc{HAssign}
+@{thm[mode=Rule] Assign} \sc{Assign}
 \end{framed}
-\caption{Assignment rules}
+\caption{The assignment rule}
 \label{fig:com}
 \end{figure}
 \<close>
@@ -75,53 +67,101 @@ text \<open>The following lemmas show that the execution of the commands is dete
 definition final :: "config \<Rightarrow> bool" where
   "final cfg \<longleftrightarrow> (case cfg of (_, _, Skip) \<Rightarrow> True | _ \<Rightarrow> False)"
 
-definition stuck :: "config \<Rightarrow> bool" where
-  "stuck cfg \<longleftrightarrow> (case cfg of
+definition stuck :: "gamma \<Rightarrow> config \<Rightarrow> bool" where
+  "stuck \<Gamma> cfg \<longleftrightarrow> (case cfg of
      (_, _, Skip) \<Rightarrow> False |
-     _ \<Rightarrow> \<not>(\<exists>cfg'. cfg \<rightarrow> cfg'))"
+     _ \<Rightarrow> \<not>(\<exists>cfg'. (\<Gamma> \<turnstile> cfg \<rightarrow> cfg')))"
 
-lemma skip_final_noteq[simp]: "(\<Gamma>, H, c) \<rightarrow> (\<Gamma>', H', c') \<Longrightarrow> c \<noteq> Skip"
+lemma skip_final_noteq[simp]: "\<Gamma> \<turnstile> (T, H, c) \<rightarrow> (T, H', c') \<Longrightarrow> c \<noteq> Skip"
 proof (cases rule: com_sem_cases)
 qed auto
 
-lemma skip_final[simp]: "\<not>(\<Gamma>, H, Skip) \<rightarrow> (\<Gamma>', H', c)"
-proof
-  assume "(\<Gamma>, H, Skip) \<rightarrow> (\<Gamma>', H', c)"
-  thus False using skip_final_noteq by blast
-qed
+lemma skip_final[simp]: "\<Gamma> \<turnstile> (T, H, Skip) \<rightarrow> (T', H', c) \<Longrightarrow> False"
+proof (cases \<Gamma> "(T, H, Skip)" "(T', H', c)" rule: com_sem_cases)
+qed auto
 
-lemma com_sem_deterministic: "cfg \<rightarrow> cfg' \<Longrightarrow> cfg \<rightarrow> cfg'' \<Longrightarrow> cfg'' = cfg'"
+lemma com_sem_det: "\<Gamma> \<turnstile> cfg \<rightarrow> cfg' \<Longrightarrow> \<Gamma> \<turnstile> cfg \<rightarrow> cfg'' \<Longrightarrow> cfg'' = cfg'"
 proof (induction arbitrary: cfg'' rule: com_sem.induct)
-  case (VAssign \<Gamma> H e H' v x)
+  case (Assign \<Gamma> H p refs a t H' T rv T' H'' v uu ts)
+  show ?case
+  proof (rule ComE(1))
+    show "\<Gamma> \<turnstile> (T, H, p ::= rv) \<rightarrow> cfg''" using Assign.prems by simp
+  next
+    fix refsa aa ta T'a H''a va uuu tsa
+
+    assume "\<Gamma>; H \<turnstile> p \<Down>\<^sub>p (refsa, Reference aa ta)"
+    then have "refsa = refs \<and> aa = a \<and> ta = t" using Assign.hyps place_sem_det' by blast
+    then have refs: "refsa = refs" and "aa = a" and "ta = t" by auto
+
+    moreover
+    assume "(\<Gamma>, T, kill_all refsa H, rv) \<Down> (T'a, H''a, va)"
+    then have "(\<Gamma>, T, H', rv) \<Down> (T'a, H''a, va)" using Assign.hyps refs by simp
+    then have "T'a = T' \<and> H''a = H'' \<and> va = v" using Assign.hyps rvalue_sem_det by blast
+    then have "T'a = T'" and "H''a = H''" and "va = v" by auto
+
+    moreover
+    assume "H''a ! aa = (uuu, tsa)"
+    then have "tsa = ts" using \<open>H''a = H''\<close> \<open>aa = a\<close> Assign.hyps by auto
+
+    moreover
+    assume "cfg'' = (T'a, H''a[aa := (va, kill ta tsa)], Skip)"
+    then show ?thesis using calculation by auto
+  qed
+next
+  case (SeqL \<Gamma> T H c)
   then show ?case
-    using exp_sem_deterministic by auto
+    by (meson ComE(3) skip_final)
 next
-  case (HAssign \<Gamma> H e\<^sub>l H' p t e\<^sub>v H'' v)
+  case (SeqR \<Gamma> T H c1 T' H' c' c2)
   then show ?case
-    by (smt ComE(2) Pair_inject exp_sem_deterministic val.inject(3))
+    by (metis ComE(3) old.prod.inject skip_final)
 next
-  case (SeqL \<Gamma> H c)
-  then show ?case using skip_final by auto
+  case (IfTrue \<Gamma> T H b T' H' c1 c2)
+  show ?case
+  proof (rule ComE(4))
+    show "\<Gamma> \<turnstile> (T, H, IF b THEN c1 ELSE c2) \<rightarrow> cfg''" using IfTrue.prems by simp
+  next
+    fix T'a H'a
+    assume "(\<Gamma>, T, H, b) \<Down> (T'a, H'a, VBool True)"
+    then have "T'a = T'" and "H'a = H'" using rvalue_sem_det IfTrue.hyps by auto
+
+    assume "cfg'' = (T'a, H'a, c1)"
+    thus ?thesis using \<open>T'a = T'\<close> \<open>H'a = H'\<close> by simp
+  next
+    fix T'a H'a
+    assume "(\<Gamma>, T, H, b) \<Down> (T'a, H'a, VBool False)"
+    then have False using rvalue_sem_det IfTrue.hyps by blast
+    thus ?thesis by simp
+  qed
 next
-  case (SeqR \<Gamma> H c1 \<Gamma>' H' c' c2)
-  then show ?case by (metis ComE(4) prod.inject skip_final)
+  case (IfFalse \<Gamma> T H b T' H' c1 c2)
+  show ?case
+  proof (rule ComE(4))
+    show "\<Gamma> \<turnstile> (T, H, IF b THEN c1 ELSE c2) \<rightarrow> cfg''" using IfFalse.prems by simp
+  next
+    fix T'a H'a
+    assume "(\<Gamma>, T, H, b) \<Down> (T'a, H'a, VBool False)"
+    then have "T'a = T'" and "H'a = H'" using rvalue_sem_det IfFalse.hyps by auto
+
+    assume "cfg'' = (T'a, H'a, c2)"
+    thus ?thesis using \<open>T'a = T'\<close> \<open>H'a = H'\<close> by simp
+  next
+    fix T'a H'a
+    assume "(\<Gamma>, T, H, b) \<Down> (T'a, H'a, VBool True)"
+    then have False using rvalue_sem_det IfFalse.hyps by blast
+    thus ?thesis by simp
+  qed
 next
-  case (IfTrue \<Gamma> H b H' c1 c2)
-then show ?case using exp_sem_deterministic by fastforce
-next
-  case (IfFlase \<Gamma> H b H' c1 c2)
-then show ?case using exp_sem_deterministic by fastforce
-next
-  case (While \<Gamma> H b c)
+  case (While \<Gamma> T H b c)
   then show ?case by auto
 qed
 
-lemmas star_induct' = star.induct[of "(\<rightarrow>)", split_format(complete)] \<^marker>\<open>tag invisible\<close>
+lemmas star_induct' = star.induct[of "com_sem \<Gamma>", split_format(complete)] \<^marker>\<open>tag invisible\<close>
 
 text \<open>We show the transitivity of @{const com_sem_steps}.\<close>
 
 lemma com_seql_trans:
-  "(\<Gamma>, H, c1) \<rightarrow>\<^sup>* (\<Gamma>', H', c1') \<Longrightarrow> (\<Gamma>, H, c1;; c2) \<rightarrow>\<^sup>* (\<Gamma>', H', c1';; c2)"
+  "\<Gamma> \<turnstile> (T, H, c1) \<rightarrow>\<^sup>* (T', H', c1') \<Longrightarrow> \<Gamma> \<turnstile> (T, H, c1;; c2) \<rightarrow>\<^sup>* (T', H', c1';; c2)"
 proof (induction rule: star_induct')
   case (refl a a b)
   then show ?case by simp
@@ -131,6 +171,37 @@ next
 qed
 
 section \<open>Code examples\<close>
+
+text \<open>We need to assign a pre-allocated location to each variable to run a program.
+Currently we initialize those locations with zeros, but they will be uninitialized when we implement
+uninitialized slots.\<close>
+
+abbreviation "\<Gamma>\<^sub>0 == \<lambda>_. undefined"
+fun preallocate' :: "vname list \<Rightarrow> gamma * tags * heap \<Rightarrow> gamma * tags * heap" where
+  "preallocate' [] ret = ret" |
+  "preallocate' (x # xs) (\<Gamma>, T, H) =
+    (let t = length T in
+     let \<Gamma>' = \<Gamma>(x := (t, t)) in
+     let T' = T @ [Unique] in
+     let H' = H @ [(VInt 0, [t])] in
+     preallocate' xs (\<Gamma>', T', H'))"
+fun preallocate :: "vname list \<Rightarrow> gamma * tags * heap" where
+  "preallocate xs = preallocate' xs (\<Gamma>\<^sub>0, [], [])"
+
+value "preallocate [''x'', ''y'']"
+value "map (fst (preallocate [''x'', ''y''])) [''x'', ''y'']"
+
+fun prealloc_com_sem :: "vname list \<Rightarrow> com \<Rightarrow> config \<Rightarrow> bool"
+  ("(_; _ \<rightarrow>\<^sup>* _)") where
+  "(xs; c \<rightarrow>\<^sup>* cfg) =
+   (let (\<Gamma>, T, H) = preallocate xs in (\<Gamma> \<turnstile> (T, H, c) \<rightarrow>\<^sup>* cfg))"
+
+text \<open>Let Isabelle run Unique programs by generating code for the semantics.\<close>
+
+code_pred [show_modes] place_sem .
+code_pred [show_modes] operand_sem .
+code_pred [show_modes] rvalue_sem .
+code_pred [show_modes] com_sem .
 
 subsection \<open>Invalidating a reference\<close>
 
@@ -157,35 +228,41 @@ The following command is the translation of the program above without the last c
 
 definition XY :: com where
   "XY =
-    ''root'' ::= Box (Const (VInt 42));;
-    ''px'' ::= Reborrow (Var ''root'');;
-    *(Var ''px'') ::= Const (VInt 100);;
-    ''py'' ::= Reborrow (Var ''root'');;
-    *(Var ''py'') ::= Const (VInt 200)"
+    (Var ''root'') ::= (Use \<circ> Constant \<circ> VInt) 42;;
+    (Var ''px'') ::= (Reborrow \<circ> Var) ''root'';;
+    ((Deref \<circ> Var) ''px'') ::= (Use \<circ> Constant \<circ> VInt) 100;;
+    (Var ''py'') ::= (Reborrow \<circ> Var) ''root'';;
+    ((Deref \<circ> Var) ''py'') ::= (Use \<circ> Constant \<circ> VInt) 200"
 
 text \<open>We can let Isabelle compute the program.\<close>
 
-values "{(map \<Gamma> [''root'', ''px'', ''py''], H, c) |
-         \<Gamma> H c. (Map.empty, [], XY) \<rightarrow>\<^sup>* (\<Gamma>, H, c)}"
+value "preallocate [''root'', ''px'', ''py'']"
+abbreviation "\<Gamma> == \<Gamma>\<^sub>0(''root'' := (0, 0), ''px'' := (1, 1), ''py'' := (2, 2))"
+abbreviation "T == [Unique, Unique, Unique]"
+abbreviation "H == [(VInt 0, [0]), (VInt 0, [1]), (VInt 0, [2])]"
+lemma "preallocate [''root'', ''px'', ''py''] = (\<Gamma>, T, H)" by auto
 
-text \<open>The following shows the variable environment and the heap at the end of execution.\<close>
+values "{(T', H') |
+         T' H' c'. \<Gamma> \<turnstile> (T, H, XY) \<rightarrow>\<^sup>* (T', H', c')}"
 
-abbreviation \<Gamma>\<^sub>X\<^sub>Y :: gamma where
-  "\<Gamma>\<^sub>X\<^sub>Y == [''root'' \<mapsto> Reference 0 1, ''px'' \<mapsto> Reference 0 2, ''py'' \<mapsto> Reference 0 3]"
+text \<open>The following shows the tags and the heap at the end of execution.\<close>
+
+abbreviation T\<^sub>X\<^sub>Y :: tags where
+  "T\<^sub>X\<^sub>Y == [Unique, Unique, Unique, Unique, Unique]" (* 5 variables + 2 reborrows *)
 abbreviation H\<^sub>X\<^sub>Y :: heap where
-  "H\<^sub>X\<^sub>Y == [(VInt 200, [1, 3])]"
+  "H\<^sub>X\<^sub>Y == [(VInt 200, [0, 4]), (Reference 0 3, [1]), (Reference 0 4, [2])]"
 
 text \<open>We can also prove that the program result in the state shown above in theory,
 but it's really tedious (why can't Isabelle prove it by computing the execution?).
 The actual proof is left to the reader.\<close>
 
-lemma final_xy: "(Map.empty, [], XY) \<rightarrow>\<^sup>* (\<Gamma>\<^sub>X\<^sub>Y, H\<^sub>X\<^sub>Y, Skip)"
+lemma final_xy: "\<Gamma> \<turnstile> (T, H, XY) \<rightarrow>\<^sup>* (T\<^sub>X\<^sub>Y, H\<^sub>X\<^sub>Y, Skip)"
   sorry \<^marker>\<open>tag important\<close>
 
 text \<open>We show that accessing through \rust{px} after the program will stuck.\<close>
 
-lemma intermediate_xyx: "(Map.empty, [], XY;; *(Var ''px'') ::= Const (VInt 300)) \<rightarrow>\<^sup>*
-  (\<Gamma>\<^sub>X\<^sub>Y, H\<^sub>X\<^sub>Y, *(Var ''px'') ::= Const (VInt 300))"
+lemma intermediate_xyx: "\<Gamma> \<turnstile> (T, H, XY;; ((Deref \<circ> Var) ''px'') ::= (Use \<circ> Constant \<circ> VInt) 300)
+  \<rightarrow>\<^sup>* (T\<^sub>X\<^sub>Y, H\<^sub>X\<^sub>Y, ((Deref \<circ> Var) ''px'') ::= (Use \<circ> Constant \<circ> VInt) 300)"
   apply (rule star_trans)
    prefer 2
    apply (rule star_step1)
@@ -194,8 +271,8 @@ lemma intermediate_xyx: "(Map.empty, [], XY;; *(Var ''px'') ::= Const (VInt 300)
   apply (rule final_xy)
   done
 
-lemma stuck_xyx: "stuck
-   (\<Gamma>\<^sub>X\<^sub>Y, H\<^sub>X\<^sub>Y, *(Var ''px'') ::= Const (VInt 300))"
+lemma stuck_xyx: "stuck \<Gamma>
+   (T\<^sub>X\<^sub>Y, H\<^sub>X\<^sub>Y, ((Deref \<circ> Var) ''px'') ::= (Use \<circ> Constant \<circ> VInt) 300)"
   apply (simp add: stuck_def)
   apply (rule allI)+
   apply (rule notI)
@@ -203,8 +280,8 @@ lemma stuck_xyx: "stuck
    apply (auto)
   done
 
-lemma "\<exists>cfg. (Map.empty, [], XY;; *(Var ''px'') ::= Const (VInt 300)) \<rightarrow>\<^sup>* cfg
-           \<and> stuck cfg"
+lemma "\<exists>cfg. (\<Gamma> \<turnstile> (T, H, XY;; ((Deref \<circ> Var) ''px'') ::= (Use \<circ> Constant \<circ> VInt) 300) \<rightarrow>\<^sup>* cfg)
+           \<and> stuck \<Gamma> cfg"
   apply (rule exI)
   apply (rule conjI)
    apply (rule intermediate_xyx)
@@ -215,17 +292,21 @@ subsection \<open>Swap\<close>
 
 text \<open>The following program swaps the content the given two references pointing to.\<close>
 
-fun swap :: "exp \<Rightarrow> exp \<Rightarrow> com" where
+fun swap :: "place \<Rightarrow> place \<Rightarrow> com" where
   "swap x y =
-    ''reborrow_x'' ::= Reborrow x;;
-    ''reborrow_y'' ::= Reborrow y;;
-    ''tmp'' ::= Deref (Var ''reborrow_x'');;
-    *(Var ''reborrow_x'') ::= Deref (Var ''reborrow_y'');;
-    *(Var ''reborrow_y'') ::= Var ''tmp''"
+    (Var ''reborrow_x'') ::= Reborrow x;;
+    (Var ''reborrow_y'') ::= Reborrow y;;
+    (Var ''tmp'') ::= (Use \<circ> Place \<circ> Deref \<circ> Deref \<circ> Var) ''reborrow_x'';;
+    ((Deref \<circ> Var) ''reborrow_x'') ::= (Use \<circ> Place \<circ> Deref \<circ> Deref \<circ> Var) ''reborrow_y'';;
+    ((Deref \<circ> Var) ''reborrow_y'') ::= (Use \<circ> Place \<circ> Deref \<circ> Deref \<circ> Var) ''tmp''"
 
 text \<open>We can see the content swapped during the execution by running it on Isabelle.\<close>
 
-values "{H | \<Gamma> H c. (Map.empty, [], swap (Box (Const (VInt 42))) (Box (Const (VInt 100)))) \<rightarrow>\<^sup>* (\<Gamma>, H, c)}"
+values "{H | T H c.
+  \<Gamma>\<^sub>0(''reborrow_x'' := (0, 0), ''reborrow_y'' := (1, 1), ''tmp'' := (2, 2), ''a'' := (3, 3), ''b'' := (4, 4)) \<turnstile>
+  ([Unique, Unique, Unique],
+   [(VInt 0, [0]), (VInt 0, [1]), (VInt 0, [2]), (VInt 10000, [3]), (VInt 20000, [4])],
+   swap (Var ''a'') (Var ''b'')) \<rightarrow>\<^sup>* (T, H, c)}"
 
 text \<open>Proving the correctness of @{const swap} would need a Hoare Logic. The road continues...\<close>
 
