CHANGELOG.md
@@ -1,5 +1,24 @@
 # Unreleased
 
+# 2020/05/13 "The Great MIRification"
+## Added
+
+- Added `tag_kind` type denotes the type of a reference. Currently `Unique` only
+- Added `tags` which tracks issued tags
+
+## Changed
+
+- Expression types now mimic MIR's ones (`exp` -> `place`, `operand`, `rvalue`)
+  - In particular, `rvalue` became non-recursive
+- Variables now refer to a memory location, and the variable context is fixed throughout the execution
+  - You need to pre-allocate a location for each variable in the program
+
+## Learned
+
+- How to use rule inversions
+  - Do NOT trust auto-generated `then show ?case`. If you are going to perform a complicated case analysis, removing `then` is a good idea
+  - I wonder why Isabelle doesn't let us assume equivalent-but-simpler propositions while proving via rule inversions
+
 # 2020/05/06
 ## Added
 
@@ -7,3 +26,4 @@
   - Big-step semantics of expressions with side-effects
   - Small-step semantics of commands
 - Example: shows XYX reference is invalid
+- Example: swap
